Some examples.

my_simple.v
@@ -2,6 +2,7 @@
 
 Require Import String List.
 Import ListNotations. Open Scope string_scope.
+Require Import Coq.Program.Basics.
 
 (* 1. Types *)
 Inductive type : Type :=
@@ -15,67 +16,81 @@ Inductive term: Type :=
 
 Definition Context := list (string * type).
 Fixpoint lookup (x : string) (Gamma : Context) : option type :=
-  match Gamma with
-  | [] => None
-  | (y, T) :: rest => if string_dec x y then Some T else lookup x rest
-  end.
+    match Gamma with 
+    | [] => None
+    | (y, T) :: rest => if string_dec x y then Some T else lookup x rest
+    end.
 
+Section TestScope.
+    Let A := Base "A".
+    Example test_lookup_found : lookup "x" [("x",  Arrow A A)] = Some (Arrow A A) := eq_refl.
+    Example test_lookup_missing : lookup "x" [("y",  Arrow A A)] = None := eq_refl.
+End TestScope.
+
+(* To understand later.*)
+Lemma type_neq_arrow : forall T U, T <> Arrow T U.
+Proof.
+  (* We use induction on the structure of T *)
+  induction T; intros U H.
+
+  - (* Case 1: T is Base s *)
+    (* H : Base s = Arrow (Base s) U *)
+    (* Here, the constructors 'Base' and 'Arrow' are different. *)
+    (* discriminate works here! *)
+    discriminate H.
+
+  - (* Case 2: T is Arrow T1 T2 *)
+    (* H : Arrow T1 T2 = Arrow (Arrow T1 T2) U *)
+    (* The constructors are BOTH 'Arrow', so discriminate FAILS here. *)
+    (* Instead, we use 'injection' to peel off the Arrow wrapper. *)
+    injection H as H1 H2.
+    
+    (* H1 : T1 = Arrow T1 T2 *)
+    (* Now we have a smaller loop! We can use the Induction Hypothesis (IHT1). *)
+    apply IHT1 in H1.
+    
+    (* H1 is now False, so we are done. *)
+    contradiction.
+Qed.
+
+  
 Inductive has_type : Context -> term -> type -> Prop :=
-  | T_Var : forall Gamma x T, lookup x Gamma = Some T -> has_type Gamma (var x) T
-  | T_Abs : forall Gamma x T1 T2 t, has_type ((x, T1) :: Gamma) t T2 -> has_type Gamma (abs x T1 t) (Arrow T1 T2)
-  | T_App : forall Gamma t1 t2 T11 T12, has_type Gamma t1 (Arrow T11 T12) -> has_type Gamma t2 T11 -> has_type Gamma (app t1 t2) T12.
+| T_Var : forall Gamma x T, lookup x Gamma = Some T -> has_type Gamma (var x) T
+| T_Abs : forall Gamma x T1 T2 t, has_type ((x, T1) :: Gamma) t T2 -> has_type Gamma (abs x T1 t) (Arrow T1 T2)
+| T_App : forall Gamma t1 t2 T11 T12, has_type Gamma t1 (Arrow T11 T12) -> has_type Gamma t2 T11 -> has_type Gamma (app t1 t2) T12.
+
+Section TestScope.
+    Let A := Base "A".
+    Let B := Base "B".
+    Let C := Base "C".
+
+    Example test_var : has_type [("x",  Arrow A A)] (var "x") (Arrow A A).
+        Proof. repeat constructor. Qed.
+   
+    Let IdentityFunction := abs "y" A (var "y").
+    Example test_id : has_type [] IdentityFunction (Arrow A A).
+        Proof. repeat constructor. Qed.
+
+    Let Second := abs "f" (Arrow A A) (abs "x" A ( app (var "f") (app (var "f") (var "x")))).
+    Example second_typeable : has_type [] Second (Arrow (Arrow A A) (Arrow A A)).
+        Proof. repeat (econstructor; try reflexivity). Qed.
+    
+    Let K := abs "x" A (abs "y" B (var "x")). 
+    Example K_typeable : has_type [] K (Arrow A (Arrow B A)).
+    Proof. repeat (econstructor; try reflexivity). Qed.
+    
+    Let Comp := abs "f" (Arrow B C) (
+                abs "g" (Arrow A B) (
+                abs "x" A (app (var "f") (app (var "g") (var "x") ))
+        )).
+    Example test_comp: has_type [] Comp (Arrow (Arrow B C) (Arrow (Arrow A B) (Arrow A C))).
+    (* (Arrow (Arrow B C) (Arrow (Arrow A B) (Arrow A C))) *)
+    Proof. repeat (econstructor; try reflexivity). Qed.
+End TestScope.
 
 Definition A := Base "A".
 Definition B := Base "B".
 Definition C := Base "C".
-
-Definition my_context := [("x", A)].
-Lemma has_type_test : has_type my_context (var "x") A.
-Proof.
-    unfold my_context.
-    apply T_Var. 
-    reflexivity.
-Qed.
-
-Definition IdentityFunction := abs "y" A (var "y").
-Lemma identity : has_type [] IdentityFunction (Arrow A A).
-Proof.
-    unfold IdentityFunction.
-    apply T_Abs.
-    apply T_Var.
-    reflexivity.
-
-Definition Second := abs "f" (Arrow A A) (abs "x" A ( app (var "f") (app (var "f") (var "x")))).
-Lemma second_typeable : has_type [] Second (Arrow (Arrow A A) (Arrow A A)).
-Proof.
-  apply T_Abs.
-  apply T_Abs.
-  eapply T_App.
-  - apply T_Var. reflexivity.
-  - eapply T_App; apply T_Var. reflexivity.
-
-Definition K := abs "x" A (abs "y" B (var "x")). 
-Lemma K_typeable : has_type [] K (Arrow A (Arrow B A)).
-Proof.
-    apply T_Abs. apply T_Abs. apply T_Var. auto.
-Qed.
-
-Definition Comp := abs "f" (Arrow B C) (
-    abs "g" (Arrow A B) (
-        abs "x" A (
-        app (var "f") (
-            app (var "g") (var "x")
-        )
-        )
-        )
-        ).
-Lemma Comp_typeable: has_type [] Comp (Arrow (Arrow B C) (Arrow (Arrow A B) (Arrow A C))).
-Proof.
-    apply T_Abs. apply T_Abs. apply T_Abs. eapply T_App. 
-    - now apply T_Var. 
-    -  eapply T_App; now apply T_Var. 
-Qed.
-
 
 (*     
 (* Types *)
